src/Init/Control/Lawful/MonadAttach/Lemmas.lean
@@ -7,6 +7,7 @@ module
 
 prelude
 public import Init.Control.MonadAttach
+import all Init.Control.MonadAttach
 public import Init.Control.Lawful.Lemmas
 public import Init.Control.Lawful.MonadLift.Lemmas
 
@@ -53,3 +54,38 @@ public theorem LawfulMonadAttach.canReturn_liftM_imp'
   intro h
   simp only [← LawfulMonadAttach.map_attach (x := x), liftM_map] at h
   exact canReturn_map_imp h
+
+public theorem LawfulMonadAttach.attach_bind_val
+    [Monad m] [MonadAttach m] [LawfulMonad m] [LawfulMonadAttach m]
+    {x : m α} {f : α → m β} :
+    MonadAttach.attach x >>= (fun a => f a.val) = x >>= f := by
+  conv => rhs; simp only [← map_attach (x := x), bind_map_left]
+
+public theorem LawfulMonadAttach.some_map_inj_iff
+    [Monad m] [MonadAttach m] [LawfulMonad m] [LawfulMonadAttach m]
+    {x y : m α} :
+    some <$> x = some <$> y ↔ x = y := by
+  apply Iff.intro
+  · exact LawfulMonadAttach.map_some_inj
+  · simp
+
+public theorem LawfulMonadAttach.bind_attach_of_nonempty
+    [Monad m] [MonadAttach m] [LawfulMonad m] [LawfulMonadAttach m] [Nonempty (m β)]
+    {x : m α} {f : Subtype (MonadAttach.CanReturn x) → m β} :
+    open scoped Classical in
+    MonadAttach.attach x >>= f = x >>= (fun a => if ha : MonadAttach.CanReturn x a then f ⟨a, ha⟩ else Classical.ofNonempty) := by
+  conv => rhs; simp +singlePass only [← LawfulMonadAttach.map_attach (x := x)]
+  simp [Subtype.property]
+
+public theorem LawfulMonadAttach.attach_bind_eq_pbind
+    [Monad m] [MonadAttach m] [LawfulMonad m] [LawfulMonadAttach m]
+    {x : m α} {f : Subtype (MonadAttach.CanReturn x) → m β} :
+    MonadAttach.attach x >>= f = MonadAttach.pbind x (fun a ha => f ⟨a, ha⟩) := by
+  simp [MonadAttach.pbind]
+
+public theorem LawfulMonadAttach.pbind_eq_bind
+    [Monad m] [MonadAttach m] [LawfulMonad m] [LawfulMonadAttach m]
+    {x : m α} {f : α → m β} :
+    MonadAttach.pbind x (fun a _ => f a) = x >>= f := by
+  conv => rhs; rw [← map_attach (x := x)]
+  simp [MonadAttach.pbind]
