src/Init/Data/Iterators/Lemmas/Combinators/Monadic/FilterMap.lean
@@ -9,6 +9,7 @@ prelude
 public import Init.Data.Iterators.Combinators.Monadic.FilterMap
 public import Init.Data.Iterators.Lemmas.Consumers.Monadic
 import all Init.Data.Iterators.Consumers.Monadic.Collect
+import Init.Control.Lawful.MonadAttach.Lemmas
 
 public section
 
@@ -92,15 +93,15 @@ theorem IterM.step_mapWithPostcondition {γ : Type w} {f : β → PostconditionT
   | .done h => rfl
 
 theorem IterM.step_filterMapM {f : β → n (Option β')}
-    [Monad n] [LawfulMonad n] [MonadLiftT m n] :
+    [Monad n] [MonadAttach n] [LawfulMonad n] [MonadLiftT m n] :
   (it.filterMapM f).step = (do
     match (← it.step).inflate with
     | .yield it' out h => do
-      match ← f out with
-      | none =>
-        pure <| .deflate <| .skip (it'.filterMapM f) (.yieldNone (out := out) h .intro)
-      | some out' =>
-        pure <| .deflate <| .yield (it'.filterMapM f) out' (.yieldSome (out := out) h .intro)
+      match ← MonadAttach.attach (f out) with
+      | ⟨none, hf⟩ =>
+        pure <| .deflate <| .skip (it'.filterMapM f) (.yieldNone (out := out) h hf)
+      | ⟨some out', hf⟩ =>
+        pure <| .deflate <| .yield (it'.filterMapM f) out' (.yieldSome (out := out) h hf)
     | .skip it' h =>
       pure <| .deflate <| .skip (it'.filterMapM f) (.skip h)
     | .done h =>
@@ -109,7 +110,6 @@ theorem IterM.step_filterMapM {f : β → n (Option β')}
   intro step
   match step.inflate with
   | .yield it' out h =>
-    simp only [PostconditionT.lift, bind_map_left]
     apply bind_congr
     intro step
     rcases step with _ | _ <;> rfl
@@ -117,15 +117,15 @@ theorem IterM.step_filterMapM {f : β → n (Option β')}
   | .done h => rfl
 
 theorem IterM.step_filterM {f : β → n (ULift Bool)}
-    [Monad n] [LawfulMonad n] [MonadLiftT m n] :
+    [Monad n] [MonadAttach n] [LawfulMonad n] [MonadLiftT m n] :
   (it.filterM f).step = (do
     match (← it.step).inflate with
     | .yield it' out h => do
-      match ← f out with
-      | .up false =>
-        pure <| .deflate <| .skip (it'.filterM f) (.yieldNone (out := out) h ⟨⟨.up false, .intro⟩, rfl⟩)
-      | .up true =>
-        pure <| .deflate <| .yield (it'.filterM f) out (.yieldSome (out := out) h ⟨⟨.up true, .intro⟩, rfl⟩)
+      match ← MonadAttach.attach (f out) with
+      | ⟨.up false, hf⟩ =>
+        pure <| .deflate <| .skip (it'.filterM f) (.yieldNone (out := out) h ⟨⟨.up false, hf⟩, rfl⟩)
+      | ⟨.up true, hf⟩ =>
+        pure <| .deflate <| .yield (it'.filterM f) out (.yieldSome (out := out) h ⟨⟨.up true, hf⟩, rfl⟩)
     | .skip it' h =>
       pure <| .deflate <| .skip (it'.filterM f) (.skip h)
     | .done h =>
@@ -134,8 +134,8 @@ theorem IterM.step_filterM {f : β → n (ULift Bool)}
   intro step
   match step.inflate with
   | .yield it' out h =>
-    simp only [PostconditionT.lift, PostconditionT.operation_map, Functor.map_map,
-      PlausibleIterStep.skip, PlausibleIterStep.yield, bind_map_left]
+    simp only [PostconditionT.operation_map, PlausibleIterStep.skip, PlausibleIterStep.yield,
+      bind_map_left]
     apply bind_congr
     intro step
     rcases step with _ | _ <;> rfl
@@ -143,12 +143,12 @@ theorem IterM.step_filterM {f : β → n (ULift Bool)}
   | .done h => rfl
 
 theorem IterM.step_mapM {γ : Type w} {f : β → n γ}
-    [Monad n] [LawfulMonad n] [MonadLiftT m n] :
+    [Monad n] [MonadAttach n] [LawfulMonad n] [MonadLiftT m n] :
   (it.mapM f).step = (do
     match (← it.step).inflate with
     | .yield it' out h => do
-      let out' ← f out
-      pure <| .deflate <| .yield (it'.mapM f) out' (.yieldSome h ⟨⟨out', True.intro⟩, rfl⟩)
+      let out' ← MonadAttach.attach (f out)
+      pure <| .deflate <| .yield (it'.mapM f) out'.val (.yieldSome h ⟨out', rfl⟩)
     | .skip it' h =>
       pure <| .deflate <| .skip (it'.mapM f) (.skip h)
     | .done h =>
@@ -158,8 +158,7 @@ theorem IterM.step_mapM {γ : Type w} {f : β → n γ}
   match step.inflate with
   | .yield it' out h =>
     simp only [bind_pure_comp]
-    simp only [PostconditionT.lift]
-    simp only [PostconditionT.operation_map, Functor.map_map, PlausibleIterStep.skip,
+    simp only [PostconditionT.operation_map, PlausibleIterStep.skip,
       PlausibleIterStep.yield, bind_map_left, bind_pure_comp]
     rfl
   | .skip it' h => rfl
@@ -293,18 +292,25 @@ theorem IterM.InternalConsumers.toList_filterMap {α β γ: Type w} {m : Type w 
   · simp
 
 theorem IterM.toList_map_eq_toList_mapM {α β γ : Type w}
-    {m : Type w → Type w'} [Monad m] [LawfulMonad m]
+    {m : Type w → Type w'} [Monad m] [MonadAttach m] [LawfulMonad m] [LawfulMonadAttach m]
     [Iterator α m β] [Finite α m] [IteratorCollect α m m] [LawfulIteratorCollect α m m]
     {f : β → γ} {it : IterM (α := α) m β} :
     (it.map f).toList = (it.mapM fun b => pure (f b)).toList := by
   induction it using IterM.inductSteps with | step it ihy ihs
   rw [toList_eq_match_step, toList_eq_match_step, step_map, step_mapM, bind_assoc, bind_assoc]
   apply bind_congr; intro step
-  split <;> simp (discharger := assumption) [ihy, ihs]
+  split
+  · simp only [PlausibleIterStep.yield, bind_pure_comp, pure_bind, Shrink.inflate_deflate,
+      bind_map_left]
+    conv => rhs; rhs; ext a; rw [← pure_bind (x := a.val) (f := fun _ => _ <$> _)]
+    simp only [← bind_assoc, bind_pure_comp, LawfulMonadAttach.map_attach]
+    simp [ihy ‹_›]
+  · simp [ihs ‹_›]
+  · simp
 
 theorem IterM.toList_mapM_eq_toList_filterMapM {α β γ : Type w}
     {m : Type w → Type w'} {n : Type w → Type w''}
-    [Monad m] [LawfulMonad m] [Monad n] [LawfulMonad n]
+    [Monad m] [LawfulMonad m] [Monad n] [MonadAttach n] [LawfulMonad n] [LawfulMonadAttach n]
     [MonadLiftT m n][LawfulMonadLiftT m n]
     [Iterator α m β] [Finite α m] [IteratorCollect α m n] [LawfulIteratorCollect α m n]
     {f : β → n γ} {it : IterM (α := α) m β} :
@@ -313,10 +319,22 @@ theorem IterM.toList_mapM_eq_toList_filterMapM {α β γ : Type w}
   induction it using IterM.inductSteps with | step it ihy ihs
   rw [toList_eq_match_step, toList_eq_match_step, step_mapM, step_filterMapM, bind_assoc, bind_assoc]
   apply bind_congr; intro step
-  split <;> simp (discharger := assumption) [ihy, ihs]
+  split
+  · rename_i out _ _
+    simp only [PlausibleIterStep.yield, bind_pure_comp, bind_map_left, Shrink.inflate_deflate,
+      PlausibleIterStep.skip, bind_assoc]
+    rw [LawfulMonadAttach.bind_attach_of_nonempty]
+    rw [show ∀ g : γ → n (List γ), f out >>= g = (some <$> f out) >>= (fun a => if ha : a.isSome then g (a.get ha) else Classical.ofNonempty) by simp]
+    rw (occs := [1]) [← LawfulMonadAttach.map_attach (x := some <$> f out)]
+    simp only [dite_eq_ite, bind_map_left]
+    apply bind_congr; rintro ⟨fx, hfx⟩
+    obtain ⟨a, ha, rfl⟩ := LawfulMonadAttach.canReturn_map_imp' hfx
+    simp [ha, ihy ‹_›]
+  · simp [ihs ‹_›]
+  · simp
 
-theorem IterM.toList_map_eq_toList_filterMapM {α β γ : Type w}
-    {m : Type w → Type w'} [Monad m] [LawfulMonad m]
+theorem IterM.toList_map_eq_toList_filterMapM {α β γ : Type w} {m : Type w → Type w'}
+    [Monad m] [MonadAttach m] [LawfulMonad m] [LawfulMonadAttach m]
     [Iterator α m β] [Finite α m] [IteratorCollect α m m] [LawfulIteratorCollect α m m]
     {f : β → γ} {it : IterM (α := α) m β} :
     (it.map f).toList = (it.filterMapM fun b => pure (some (f b))).toList := by
@@ -326,7 +344,9 @@ theorem IterM.toList_map_eq_toList_filterMapM {α β γ : Type w}
 @[simp]
 theorem IterM.toList_filterMapM_filterMapM {α β γ δ : Type w}
     {m : Type w → Type w'} {n : Type w → Type w''} {o : Type w → Type w'''}
-    [Monad m] [LawfulMonad m] [Monad n] [LawfulMonad n] [Monad o] [LawfulMonad o]
+    [Monad m] [LawfulMonad m]
+    [Monad n] [MonadAttach n] [LawfulMonad n] [LawfulMonadAttach n]
+    [Monad o] [MonadAttach o] [LawfulMonad o] [LawfulMonadAttach o]
     [MonadLiftT m n] [MonadLiftT n o] [LawfulMonadLiftT m n] [LawfulMonadLiftT n o]
     [Iterator α m β] [Finite α m] [IteratorCollect α m m] [LawfulIteratorCollect α m m]
     {f : β → n (Option γ)} {g : γ → o (Option δ)}
@@ -346,10 +366,20 @@ theorem IterM.toList_filterMapM_filterMapM {α β γ δ : Type w}
   apply bind_congr; intro step
   split
   · simp only [bind_assoc, liftM_bind]
+    have {ε τ : Type _} (x : o (Option ε)) (f : (a : Option ε) → MonadAttach.CanReturn x a → o τ) :
+        MonadAttach.pbind x f = MonadAttach.pbind x (fun a ha => if h : a.isSome then f (some (a.get h)) (by simp [ha]) else f none (by simp_all)) := by
+      congr; ext a
+      cases a <;> simp +contextual
+    conv => rhs; simp only [LawfulMonadAttach.attach_bind_eq_pbind]
+    conv => rhs; rw [this]
+    simp only [bind_pure_comp, pure_bind, Shrink.inflate_deflate, LawfulMonadAttach.pbind_eq_bind,
+      bind_assoc]
+    conv => rhs; rw [← LawfulMonadAttach.map_attach (x := f _), liftM_map, bind_map_left]
     apply bind_congr; intro fx
     split
     · simp [ihy ‹_›]
-    · simp only [liftM_pure, PlausibleIterStep.skip, pure_bind, bind_assoc, Shrink.inflate_deflate]
+    · simp only [liftM_pure, pure_bind, bind_assoc, Shrink.inflate_deflate]
+      conv => rhs; rw [← LawfulMonadAttach.map_attach (x := g _), bind_map_left]
       apply bind_congr; intro gx
       split <;> simp [ihy ‹_›]
   · simp [ihs ‹_›]
@@ -358,7 +388,8 @@ theorem IterM.toList_filterMapM_filterMapM {α β γ δ : Type w}
 @[simp]
 theorem IterM.toList_filterMapM_mapM {α β γ δ : Type w}
     {m : Type w → Type w'} {n : Type w → Type w''} {o : Type w → Type w'''}
-    [Monad m] [LawfulMonad m] [Monad n] [LawfulMonad n] [Monad o] [LawfulMonad o]
+    [Monad m] [LawfulMonad m] [Monad n] [MonadAttach n] [LawfulMonad n] [LawfulMonadAttach n]
+    [Monad o] [MonadAttach o] [LawfulMonad o] [LawfulMonadAttach o]
     [MonadLiftT m n] [MonadLiftT n o] [LawfulMonadLiftT m n] [LawfulMonadLiftT n o]
     [Iterator α m β] [Finite α m]
     {f : β → n γ} {g : γ → o (Option δ)}
@@ -375,8 +406,17 @@ theorem IterM.toList_filterMapM_mapM {α β γ δ : Type w}
   apply bind_congr; intro step
   split
   · simp only [bind_assoc, liftM_bind]
+    conv => rhs; simp only [LawfulMonadAttach.attach_bind_eq_pbind]
+    have {ε τ : Type _} (x : o (Option ε)) (f : (a : Option ε) → MonadAttach.CanReturn x a → o τ) :
+        MonadAttach.pbind x f = MonadAttach.pbind x (fun a ha => if h : a.isSome then f (some (a.get h)) (by simp [ha]) else f none (by simp_all)) := by
+      congr; ext a
+      cases a <;> simp +contextual
+    conv => rhs; rw [this]
+    simp only [liftM_pure, bind_pure_comp, pure_bind, Shrink.inflate_deflate, bind_assoc,
+      LawfulMonadAttach.pbind_eq_bind]
+    conv => rhs; rw [← LawfulMonadAttach.map_attach (x := f _), liftM_map, bind_map_left]
     apply bind_congr; intro fx
-    simp only [liftM_pure, pure_bind, bind_assoc, Shrink.inflate_deflate]
+    conv => rhs; rw [← LawfulMonadAttach.map_attach (x := g _), bind_map_left]
     apply bind_congr; intro gx
     split <;> simp [ihy ‹_›]
   · simp [ihs ‹_›]
@@ -385,7 +425,7 @@ theorem IterM.toList_filterMapM_mapM {α β γ δ : Type w}
 @[simp]
 theorem IterM.toList_filterMapM_map {α β γ δ : Type w}
     {m : Type w → Type w'} {n : Type w → Type w''}
-    [Monad m] [LawfulMonad m] [Monad n] [LawfulMonad n]
+    [Monad m] [LawfulMonad m] [Monad n] [MonadAttach n] [LawfulMonad n] [LawfulMonadAttach n]
     [MonadLiftT m n] [LawfulMonadLiftT m n]
     [Iterator α m β] [Finite α m]
     {f : β → γ} {g : γ → n (Option δ)}
@@ -407,7 +447,8 @@ theorem IterM.toList_filterMapM_map {α β γ δ : Type w}
 @[simp]
 theorem IterM.toList_mapM_filterMapM {α β γ δ : Type w}
     {m : Type w → Type w'} {n : Type w → Type w''} {o : Type w → Type w'''}
-    [Monad m] [LawfulMonad m] [Monad n] [LawfulMonad n] [Monad o] [LawfulMonad o]
+    [Monad m] [LawfulMonad m] [Monad n] [MonadAttach n] [LawfulMonad n] [LawfulMonadAttach n]
+    [Monad o] [MonadAttach o] [LawfulMonad o] [LawfulMonadAttach o]
     [MonadLiftT m n] [MonadLiftT n o] [LawfulMonadLiftT m n] [LawfulMonadLiftT n o]
     [Iterator α m β] [Finite α m] [IteratorCollect α m m] [LawfulIteratorCollect α m m]
     {f : β → n (Option γ)} {g : γ → o δ}
@@ -423,7 +464,8 @@ theorem IterM.toList_mapM_filterMapM {α β γ δ : Type w}
 @[simp]
 theorem IterM.toList_mapM_mapM {α β γ δ : Type w}
     {m : Type w → Type w'} {n : Type w → Type w''} {o : Type w → Type w'''}
-    [Monad m] [LawfulMonad m] [Monad n] [LawfulMonad n] [Monad o] [LawfulMonad o]
+    [Monad m] [LawfulMonad m] [Monad n] [MonadAttach n] [LawfulMonad n] [LawfulMonadAttach n]
+    [Monad o] [MonadAttach o] [LawfulMonad o] [LawfulMonadAttach o]
     [MonadLiftT m n] [MonadLiftT n o] [LawfulMonadLiftT m n] [LawfulMonadLiftT n o]
     [Iterator α m β] [Finite α m] [IteratorCollect α m o] [LawfulIteratorCollect α m o]
     {f : β → n γ} {g : γ → o δ}
@@ -437,7 +479,7 @@ theorem IterM.toList_mapM_mapM {α β γ δ : Type w}
 @[simp]
 theorem IterM.toList_mapM_map {α β γ δ : Type w}
     {m : Type w → Type w'} {n : Type w → Type w''}
-    [Monad m] [LawfulMonad m] [Monad n] [LawfulMonad n]
+    [Monad m] [LawfulMonad m] [Monad n] [MonadAttach n] [LawfulMonad n] [LawfulMonadAttach n]
     [MonadLiftT m n] [LawfulMonadLiftT m n]
     [Iterator α m β] [Finite α m] [IteratorCollect α m n] [LawfulIteratorCollect α m n]
     {f : β → γ} {g : γ → n δ}
@@ -445,6 +487,20 @@ theorem IterM.toList_mapM_map {α β γ δ : Type w}
     ((it.map f).mapM g).toList =
       (it.mapM (n := n) (fun b => g (f b))).toList := by
   simp [toList_mapM_eq_toList_filterMapM]
+
+@[simp]
+theorem IterM.toList_map_mapM {α β γ δ : Type w}
+    {m : Type w → Type w'} {n : Type w → Type w''}
+    [Monad m] [LawfulMonad m] [Monad n] [MonadAttach n] [LawfulMonad n] [LawfulMonadAttach n]
+    [MonadLiftT m n] [LawfulMonadLiftT m n]
+    [Iterator α m β] [Finite α m] [IteratorCollect α m n] [LawfulIteratorCollect α m n]
+    {f : β → n γ} {g : γ → δ}
+    {it : IterM (α := α) m β} :
+    ((it.mapM f).map g).toList =
+      (it.mapM (n := n) (fun b => return g (← f b))).toList := by
+  simp only [toList_mapM_eq_toList_filterMapM, toList_map_eq_toList_filterMapM,
+    toList_filterMapM_mapM]
+  congr <;> simp
 
 theorem IterM.toList_filterMap {α β γ : Type w} {m : Type w → Type w'}
     [Monad m] [LawfulMonad m]
@@ -509,7 +565,7 @@ end ToList
 section ToListRev
 
 theorem IterM.toListRev_map_eq_toListRev_mapM {α β γ : Type w}
-    {m : Type w → Type w'} [Monad m] [LawfulMonad m]
+    {m : Type w → Type w'} [Monad m] [MonadAttach m] [LawfulMonad m] [LawfulMonadAttach m]
     [Iterator α m β] [Finite α m] [IteratorCollect α m m] [LawfulIteratorCollect α m m]
     {f : β → γ} {it : IterM (α := α) m β} :
     (it.map f).toListRev = (it.mapM fun b => pure (f b)).toListRev := by
@@ -517,7 +573,7 @@ theorem IterM.toListRev_map_eq_toListRev_mapM {α β γ : Type w}
 
 theorem IterM.toListRev_mapM_eq_toListRev_filterMapM {α β γ : Type w}
     {m : Type w → Type w'} {n : Type w → Type w''}
-    [Monad m] [LawfulMonad m] [Monad n] [LawfulMonad n]
+    [Monad m] [LawfulMonad m] [Monad n] [MonadAttach n] [LawfulMonad n] [LawfulMonadAttach n]
     [MonadLiftT m n][LawfulMonadLiftT m n]
     [Iterator α m β] [Finite α m] [IteratorCollect α m n] [LawfulIteratorCollect α m n]
     {f : β → n γ} {it : IterM (α := α) m β} :
@@ -526,7 +582,7 @@ theorem IterM.toListRev_mapM_eq_toListRev_filterMapM {α β γ : Type w}
   simp [toListRev_eq, toList_mapM_eq_toList_filterMapM]
 
 theorem IterM.toListRev_map_eq_toListRev_filterMapM {α β γ : Type w}
-    {m : Type w → Type w'} [Monad m] [LawfulMonad m]
+    {m : Type w → Type w'} [Monad m] [MonadAttach m] [LawfulMonad m] [LawfulMonadAttach m]
     [Iterator α m β] [Finite α m] [IteratorCollect α m m] [LawfulIteratorCollect α m m]
     {f : β → γ} {it : IterM (α := α) m β} :
     (it.map f).toListRev = (it.filterMapM fun b => pure (some (f b))).toListRev := by
@@ -554,7 +610,9 @@ theorem IterM.toListRev_filter {α β : Type w} {m : Type w → Type w'} [Monad 
 @[simp]
 theorem IterM.toListRev_filterMapM_filterMapM {α β γ δ : Type w}
     {m : Type w → Type w'} {n : Type w → Type w''} {o : Type w → Type w'''}
-    [Monad m] [LawfulMonad m] [Monad n] [LawfulMonad n] [Monad o] [LawfulMonad o]
+    [Monad m] [LawfulMonad m]
+    [Monad n] [MonadAttach n] [LawfulMonad n] [LawfulMonadAttach n]
+    [Monad o] [MonadAttach o] [LawfulMonad o] [LawfulMonadAttach o]
     [MonadLiftT m n] [MonadLiftT n o] [LawfulMonadLiftT m n] [LawfulMonadLiftT n o]
     [Iterator α m β] [Finite α m] [IteratorCollect α m m] [LawfulIteratorCollect α m m]
     {f : β → n (Option γ)} {g : γ → o (Option δ)}
@@ -570,7 +628,9 @@ theorem IterM.toListRev_filterMapM_filterMapM {α β γ δ : Type w}
 @[simp]
 theorem IterM.toListRev_filterMapM_mapM {α β γ δ : Type w}
     {m : Type w → Type w'} {n : Type w → Type w''} {o : Type w → Type w'''}
-    [Monad m] [LawfulMonad m] [Monad n] [LawfulMonad n] [Monad o] [LawfulMonad o]
+    [Monad m] [LawfulMonad m]
+    [Monad n] [MonadAttach n] [LawfulMonad n] [LawfulMonadAttach n]
+    [Monad o] [MonadAttach o] [LawfulMonad o] [LawfulMonadAttach o]
     [MonadLiftT m n] [MonadLiftT n o] [LawfulMonadLiftT m n] [LawfulMonadLiftT n o]
     [Iterator α m β] [Finite α m] [IteratorCollect α m m] [LawfulIteratorCollect α m m]
     {f : β → n γ} {g : γ → o (Option δ)}
@@ -583,7 +643,7 @@ theorem IterM.toListRev_filterMapM_mapM {α β γ δ : Type w}
 @[simp]
 theorem IterM.toListRev_filterMapM_map {α β γ δ : Type w}
     {m : Type w → Type w'} {n : Type w → Type w''}
-    [Monad m] [LawfulMonad m] [Monad n] [LawfulMonad n]
+    [Monad m] [LawfulMonad m] [Monad n] [MonadAttach n] [LawfulMonad n] [LawfulMonadAttach n]
     [MonadLiftT m n] [LawfulMonadLiftT m n]
     [Iterator α m β] [Finite α m] [IteratorCollect α m m] [LawfulIteratorCollect α m m]
     {f : β → γ} {g : γ → n (Option δ)}
@@ -595,7 +655,9 @@ theorem IterM.toListRev_filterMapM_map {α β γ δ : Type w}
 @[simp]
 theorem IterM.toListRev_mapM_filterMapM {α β γ δ : Type w}
     {m : Type w → Type w'} {n : Type w → Type w''} {o : Type w → Type w'''}
-    [Monad m] [LawfulMonad m] [Monad n] [LawfulMonad n] [Monad o] [LawfulMonad o]
+    [Monad m] [LawfulMonad m]
+    [Monad n] [MonadAttach n] [LawfulMonad n] [LawfulMonadAttach n]
+    [Monad o] [MonadAttach o] [LawfulMonad o] [LawfulMonadAttach o]
     [MonadLiftT m n] [MonadLiftT n o] [LawfulMonadLiftT m n] [LawfulMonadLiftT n o]
     [Iterator α m β] [Finite α m] [IteratorCollect α m m] [LawfulIteratorCollect α m m]
     {f : β → n (Option γ)} {g : γ → o δ}
@@ -611,7 +673,8 @@ theorem IterM.toListRev_mapM_filterMapM {α β γ δ : Type w}
 @[simp]
 theorem IterM.toListRev_mapM_mapM {α β γ δ : Type w}
     {m : Type w → Type w'} {n : Type w → Type w''} {o : Type w → Type w'''}
-    [Monad m] [LawfulMonad m] [Monad n] [LawfulMonad n] [Monad o] [LawfulMonad o]
+    [Monad m] [LawfulMonad m] [Monad n] [MonadAttach n] [LawfulMonad n] [LawfulMonadAttach n]
+    [Monad o] [MonadAttach o] [LawfulMonad o] [LawfulMonadAttach o]
     [MonadLiftT m n] [MonadLiftT n o] [LawfulMonadLiftT m n] [LawfulMonadLiftT n o]
     [Iterator α m β] [Finite α m]
     {f : β → n γ} {g : γ → o δ}
@@ -625,7 +688,7 @@ theorem IterM.toListRev_mapM_mapM {α β γ δ : Type w}
 @[simp]
 theorem IterM.toListRev_mapM_map {α β γ δ : Type w}
     {m : Type w → Type w'} {n : Type w → Type w''}
-    [Monad m] [LawfulMonad m] [Monad n] [LawfulMonad n]
+    [Monad m] [LawfulMonad m] [Monad n] [MonadAttach n] [LawfulMonad n] [LawfulMonadAttach n]
     [MonadLiftT m n] [LawfulMonadLiftT m n]
     [Iterator α m β] [Finite α m] {f : β → γ} {g : γ → n δ} {it : IterM (α := α) m β} :
     ((it.map f).mapM g).toListRev =
@@ -638,7 +701,7 @@ end ToListRev
 section ToArray
 
 theorem IterM.toArray_map_eq_toArray_mapM {α β γ : Type w}
-    {m : Type w → Type w'} [Monad m] [LawfulMonad m]
+    {m : Type w → Type w'} [Monad m] [MonadAttach m] [LawfulMonad m] [LawfulMonadAttach m]
     [Iterator α m β] [Finite α m] [IteratorCollect α m m] [LawfulIteratorCollect α m m]
     {f : β → γ} {it : IterM (α := α) m β} :
     (it.map f).toArray = (it.mapM fun b => pure (f b)).toArray := by
@@ -646,7 +709,8 @@ theorem IterM.toArray_map_eq_toArray_mapM {α β γ : Type w}
 
 theorem IterM.toArray_mapM_eq_toArray_filterMapM {α β γ : Type w}
     {m : Type w → Type w'} {n : Type w → Type w''}
-    [Monad m] [LawfulMonad m] [Monad n] [LawfulMonad n]
+    [Monad m] [LawfulMonad m]
+    [Monad n] [MonadAttach n] [LawfulMonad n] [LawfulMonadAttach n]
     [MonadLiftT m n][LawfulMonadLiftT m n]
     [Iterator α m β] [Finite α m] [IteratorCollect α m n] [LawfulIteratorCollect α m n]
     {f : β → n γ} {it : IterM (α := α) m β} :
@@ -654,7 +718,7 @@ theorem IterM.toArray_mapM_eq_toArray_filterMapM {α β γ : Type w}
   simp [← toArray_toList, toList_mapM_eq_toList_filterMapM]
 
 theorem IterM.toArray_map_eq_toArray_filterMapM {α β γ : Type w}
-    {m : Type w → Type w'} [Monad m] [LawfulMonad m]
+    {m : Type w → Type w'} [Monad m] [MonadAttach m] [LawfulMonad m] [LawfulMonadAttach m]
     [Iterator α m β] [Finite α m] [IteratorCollect α m m] [LawfulIteratorCollect α m m]
     {f : β → γ} {it : IterM (α := α) m β} :
     (it.map f).toArray = (it.filterMapM fun b => pure (some (f b))).toArray := by
@@ -682,7 +746,9 @@ theorem IterM.toArray_filter {α : Type w} {m : Type w → Type w'} [Monad m] [L
 @[simp]
 theorem IterM.toArray_filterMapM_filterMapM {α β γ δ : Type w}
     {m : Type w → Type w'} {n : Type w → Type w''} {o : Type w → Type w'''}
-    [Monad m] [LawfulMonad m] [Monad n] [LawfulMonad n] [Monad o] [LawfulMonad o]
+    [Monad m] [LawfulMonad m]
+    [Monad n] [MonadAttach n] [LawfulMonad n] [LawfulMonadAttach n]
+    [Monad o] [MonadAttach o] [LawfulMonad o] [LawfulMonadAttach o]
     [MonadLiftT m n] [MonadLiftT n o] [LawfulMonadLiftT m n] [LawfulMonadLiftT n o]
     [Iterator α m β] [Finite α m] [IteratorCollect α m m] [LawfulIteratorCollect α m m]
     {f : β → n (Option γ)} {g : γ → o (Option δ)}
@@ -698,9 +764,11 @@ theorem IterM.toArray_filterMapM_filterMapM {α β γ δ : Type w}
 @[simp]
 theorem IterM.toArray_filterMapM_mapM {α β γ δ : Type w}
     {m : Type w → Type w'} {n : Type w → Type w''} {o : Type w → Type w'''}
-    [Monad m] [LawfulMonad m] [Monad n] [LawfulMonad n] [Monad o] [LawfulMonad o]
+    [Monad m] [LawfulMonad m]
+    [Monad n] [MonadAttach n] [LawfulMonad n] [LawfulMonadAttach n]
+    [Monad o] [MonadAttach o] [LawfulMonad o] [LawfulMonadAttach o]
     [MonadLiftT m n] [MonadLiftT n o] [LawfulMonadLiftT m n] [LawfulMonadLiftT n o]
-    [Iterator α m β] [Finite α m] [IteratorCollect α m m] [LawfulIteratorCollect α m m]
+    [Iterator α m β] [Finite α m]
     {f : β → n γ} {g : γ → o (Option δ)}
     {it : IterM (α := α) m β} :
     haveI : MonadLift n o := ⟨monadLift⟩
@@ -711,7 +779,7 @@ theorem IterM.toArray_filterMapM_mapM {α β γ δ : Type w}
 @[simp]
 theorem IterM.toArray_filterMapM_map {α β γ δ : Type w}
     {m : Type w → Type w'} {n : Type w → Type w''}
-    [Monad m] [LawfulMonad m] [Monad n] [LawfulMonad n]
+    [Monad m] [LawfulMonad m] [Monad n] [MonadAttach n] [LawfulMonad n] [LawfulMonadAttach n]
     [MonadLiftT m n] [LawfulMonadLiftT m n]
     [Iterator α m β] [Finite α m] [IteratorCollect α m m] [LawfulIteratorCollect α m m]
     {f : β → γ} {g : γ → n (Option δ)}
@@ -723,7 +791,8 @@ theorem IterM.toArray_filterMapM_map {α β γ δ : Type w}
 @[simp]
 theorem IterM.toArray_mapM_filterMapM {α β γ δ : Type w}
     {m : Type w → Type w'} {n : Type w → Type w''} {o : Type w → Type w'''}
-    [Monad m] [LawfulMonad m] [Monad n] [LawfulMonad n] [Monad o] [LawfulMonad o]
+    [Monad m] [LawfulMonad m] [Monad n] [MonadAttach n] [LawfulMonad n] [LawfulMonadAttach n]
+    [Monad o] [MonadAttach o] [LawfulMonad o] [LawfulMonadAttach o]
     [MonadLiftT m n] [MonadLiftT n o] [LawfulMonadLiftT m n] [LawfulMonadLiftT n o]
     [Iterator α m β] [Finite α m] [IteratorCollect α m m] [LawfulIteratorCollect α m m]
     {f : β → n (Option γ)} {g : γ → o δ}
@@ -739,7 +808,8 @@ theorem IterM.toArray_mapM_filterMapM {α β γ δ : Type w}
 @[simp]
 theorem IterM.toArray_mapM_mapM {α β γ δ : Type w}
     {m : Type w → Type w'} {n : Type w → Type w''} {o : Type w → Type w'''}
-    [Monad m] [LawfulMonad m] [Monad n] [LawfulMonad n] [Monad o] [LawfulMonad o]
+    [Monad m] [LawfulMonad m] [Monad n] [MonadAttach n] [LawfulMonad n] [LawfulMonadAttach n]
+    [Monad o] [MonadAttach o] [LawfulMonad o] [LawfulMonadAttach o]
     [MonadLiftT m n] [MonadLiftT n o] [LawfulMonadLiftT m n] [LawfulMonadLiftT n o]
     [Iterator α m β] [Finite α m] [IteratorCollect α m o] [LawfulIteratorCollect α m o]
     {f : β → n γ} {g : γ → o δ}
@@ -752,7 +822,7 @@ theorem IterM.toArray_mapM_mapM {α β γ δ : Type w}
 @[simp]
 theorem IterM.toArray_mapM_map {α β γ δ : Type w}
     {m : Type w → Type w'} {n : Type w → Type w''}
-    [Monad m] [LawfulMonad m] [Monad n] [LawfulMonad n]
+    [Monad m] [LawfulMonad m] [Monad n] [MonadAttach n] [LawfulMonad n] [LawfulMonadAttach n]
     [MonadLiftT m n] [LawfulMonadLiftT m n]
     [Iterator α m β] [Finite α m] [IteratorCollect α m n] [LawfulIteratorCollect α m n]
     {f : β → γ} {g : γ → n δ}
@@ -761,6 +831,20 @@ theorem IterM.toArray_mapM_map {α β γ δ : Type w}
       (it.mapM (n := n) (fun b => g (f b))).toArray := by
   simp [← toArray_toList]
 
+@[simp]
+theorem IterM.toArray_map_mapM {α β γ δ : Type w}
+    {m : Type w → Type w'} {n : Type w → Type w''}
+    [Monad m] [LawfulMonad m] [Monad n] [MonadAttach n] [LawfulMonad n] [LawfulMonadAttach n]
+    [MonadLiftT m n] [LawfulMonadLiftT m n]
+    [Iterator α m β] [Finite α m] [IteratorCollect α m n] [LawfulIteratorCollect α m n]
+    {f : β → n γ} {g : γ → δ}
+    {it : IterM (α := α) m β} :
+    ((it.mapM f).map g).toArray =
+      (it.mapM (n := n) (fun b => return g (← f b))).toArray := by
+  simp only [toArray_mapM_eq_toArray_filterMapM, toArray_map_eq_toArray_filterMapM,
+    toArray_filterMapM_mapM]
+  congr <;> simp
+
 end ToArray
 
 section Fold
@@ -768,7 +852,9 @@ section Fold
 theorem IterM.foldM_filterMapM {α β γ δ : Type w}
     {m : Type w → Type w'} {n : Type w → Type w''} {o : Type w → Type w'''}
     [Iterator α m β] [Finite α m]
-    [Monad m] [Monad n] [Monad o] [LawfulMonad m] [LawfulMonad n] [LawfulMonad o]
+    [Monad m] [LawfulMonad m]
+    [Monad n] [MonadAttach n] [LawfulMonad n] [LawfulMonadAttach n]
+    [Monad o] [LawfulMonad o]
     [IteratorLoop α m n] [IteratorLoop α m o]
     [LawfulIteratorLoop α m n] [LawfulIteratorLoop α m o]
     [MonadLiftT m n] [MonadLiftT n o] [LawfulMonadLiftT m n] [LawfulMonadLiftT n o]
@@ -784,6 +870,7 @@ theorem IterM.foldM_filterMapM {α β γ δ : Type w}
   apply bind_congr; intro step
   cases step.inflate using PlausibleIterStep.casesOn
   · simp only [PlausibleIterStep.skip, PlausibleIterStep.yield, liftM_bind, bind_assoc]
+    conv => rhs; rw [← LawfulMonadAttach.map_attach (x := f _), liftM_map, bind_map_left]
     apply bind_congr; intro c?
     split <;> simp [ihy ‹_›]
   · simp [ihs ‹_›]
@@ -792,7 +879,9 @@ theorem IterM.foldM_filterMapM {α β γ δ : Type w}
 theorem IterM.foldM_mapM {α β γ δ : Type w}
     {m : Type w → Type w'} {n : Type w → Type w''} {o : Type w → Type w'''}
     [Iterator α m β] [Finite α m]
-    [Monad m] [Monad n] [Monad o] [LawfulMonad m] [LawfulMonad n] [LawfulMonad o]
+    [Monad m] [LawfulMonad m]
+    [Monad n] [MonadAttach n] [LawfulMonad n] [LawfulMonadAttach n]
+    [Monad o] [LawfulMonad o]
     [IteratorLoop α m n] [IteratorLoop α m o]
     [LawfulIteratorLoop α m n] [LawfulIteratorLoop α m o]
     [MonadLiftT m n] [MonadLiftT n o] [LawfulMonadLiftT m n] [LawfulMonadLiftT n o]
@@ -805,7 +894,9 @@ theorem IterM.foldM_mapM {α β γ δ : Type w}
   rw [foldM_eq_match_step, foldM_eq_match_step, step_mapM, liftM_bind, bind_assoc]
   apply bind_congr; intro step
   cases step.inflate using PlausibleIterStep.casesOn
-  · simp [ihy ‹_›]
+  · simp only [bind_pure_comp, liftM_map, bind_map_left, Shrink.inflate_deflate, bind_assoc]
+    conv => rhs; rw [← LawfulMonadAttach.map_attach (x := f _)]
+    simp [ihy ‹_›]
   · simp [ihs ‹_›]
   · simp
 
@@ -845,7 +936,9 @@ theorem IterM.foldM_map {α β γ δ : Type w} {m : Type w → Type w'} {n : Typ
   · simp
 
 theorem IterM.fold_filterMapM {α β γ δ : Type w} {m : Type w → Type w'} {n : Type w → Type w''}
-    [Iterator α m β] [Finite α m] [Monad m] [Monad n] [LawfulMonad m] [LawfulMonad n]
+    [Iterator α m β] [Finite α m]
+    [Monad m] [LawfulMonad m]
+    [Monad n] [MonadAttach n] [LawfulMonad n] [LawfulMonadAttach n]
     [IteratorLoop α m m] [IteratorLoop α m n]
     [LawfulIteratorLoop α m m] [LawfulIteratorLoop α m n]
     [MonadLiftT m n] [LawfulMonadLiftT m n]
@@ -857,7 +950,9 @@ theorem IterM.fold_filterMapM {α β γ δ : Type w} {m : Type w → Type w'} {n
   simp [fold_eq_foldM, foldM_filterMapM]
 
 theorem IterM.fold_mapM {α β γ δ : Type w} {m : Type w → Type w'} {n : Type w → Type w''}
-    [Iterator α m β] [Finite α m] [Monad m] [Monad n] [LawfulMonad m] [LawfulMonad n]
+    [Iterator α m β] [Finite α m]
+    [Monad m] [LawfulMonad m]
+    [Monad n] [MonadAttach n] [LawfulMonad n] [LawfulMonadAttach n]
     [IteratorLoop α m m] [IteratorLoop α m n]
     [LawfulIteratorLoop α m m] [LawfulIteratorLoop α m n]
     [MonadLiftT m n] [LawfulMonadLiftT m n]
@@ -909,8 +1004,9 @@ end Count
 section AnyAll
 
 theorem IterM.anyM_filterMapM {α β β' : Type w} {m : Type w → Type w'} {n : Type w → Type w''}
-    [Iterator α m β] [Finite α m] [Monad m] [Monad n] [MonadLiftT m n]
-    [LawfulMonad m] [LawfulMonad n]
+    [Iterator α m β] [Finite α m] [MonadLiftT m n]
+    [Monad m] [LawfulMonad m]
+    [Monad n] [MonadAttach n] [LawfulMonad n] [LawfulMonadAttach n]
     {it : IterM (α := α) m β} {f : β → n (Option β')} {p : β' → n (ULift Bool)} :
     (it.filterMapM f).anyM p = (it.mapM (pure (f := n))).anyM (fun x => do
       match ← f x with
@@ -920,7 +1016,16 @@ theorem IterM.anyM_filterMapM {α β β' : Type w} {m : Type w → Type w'} {n :
   rw [anyM_eq_match_step, anyM_eq_match_step, step_filterMapM, step_mapM, bind_assoc, bind_assoc]
   apply bind_congr; intro step
   split
-  · simp only [bind_assoc, pure_bind, Shrink.inflate_deflate]
+  · rename_i out _ _
+    simp only [bind_assoc, pure_bind, Shrink.inflate_deflate]
+    have {x : n (ULift Bool)} : x = MonadAttach.attach (pure out) >>= (fun _ => x) := by
+      rw (occs := [1]) [show x = pure out >>= (fun _ => x) by simp]
+      conv => lhs; rw [← LawfulMonadAttach.map_attach (x := pure out)]
+      simp
+    refine Eq.trans this ?_
+    simp only [LawfulMonadAttach.bind_attach_of_nonempty (x := pure out), pure_bind]
+    split; rotate_left; rfl
+    conv => rhs; rw [← LawfulMonadAttach.map_attach (x := f _), bind_map_left]
     apply bind_congr; intro fx
     split
     · simp [ihy ‹_›]
@@ -932,15 +1037,24 @@ theorem IterM.anyM_filterMapM {α β β' : Type w} {m : Type w → Type w'} {n :
   · simp
 
 theorem IterM.anyM_mapM {α β β' : Type w} {m : Type w → Type w'} {n : Type w → Type w''}
-    [Iterator α m β] [Finite α m] [Monad m] [Monad n] [MonadLiftT m n]
-    [LawfulMonad m] [LawfulMonad n]
+    [Iterator α m β] [Finite α m] [MonadLiftT m n]
+    [Monad m] [LawfulMonad m] [Monad n] [MonadAttach n] [LawfulMonad n] [LawfulMonadAttach n]
     {it : IterM (α := α) m β} {f : β → n β'} {p : β' → n (ULift Bool)} :
     (it.mapM f).anyM p = (it.mapM (pure (f := n))).anyM (fun x => do p (← f x)) := by
   induction it using IterM.inductSteps with | step it ihy ihs
   rw [anyM_eq_match_step, anyM_eq_match_step, step_mapM, step_mapM, bind_assoc, bind_assoc]
   apply bind_congr; intro step
   split
-  · simp only [bind_assoc, pure_bind, Shrink.inflate_deflate]
+  · rename_i out _ _
+    simp only [bind_assoc, pure_bind, Shrink.inflate_deflate]
+    have {x : n (ULift Bool)} : x = MonadAttach.attach (pure out) >>= (fun _ => x) := by
+      rw (occs := [1]) [show x = pure out >>= (fun _ => x) by simp]
+      conv => lhs; rw [← LawfulMonadAttach.map_attach (x := pure out)]
+      simp
+    refine Eq.trans this ?_
+    simp only [LawfulMonadAttach.bind_attach_of_nonempty (x := pure out), pure_bind]
+    split; rotate_left; rfl
+    conv => rhs; rw [← LawfulMonadAttach.map_attach (x := f _), bind_map_left]
     apply bind_congr; intro fx
     simp [ihy ‹_›]
   · simp only [PlausibleIterStep.skip, pure_bind, bind_assoc]
@@ -948,8 +1062,8 @@ theorem IterM.anyM_mapM {α β β' : Type w} {m : Type w → Type w'} {n : Type 
   · simp
 
 theorem IterM.anyM_filterM {α β : Type w} {m : Type w → Type w'} {n : Type w → Type w''}
-    [Iterator α m β] [Finite α m] [Monad m] [Monad n] [MonadLiftT m n]
-    [LawfulMonad m] [LawfulMonad n]
+    [Iterator α m β] [Finite α m] [MonadLiftT m n]
+    [Monad m] [LawfulMonad m] [Monad n] [MonadAttach n] [LawfulMonad n] [LawfulMonadAttach n]
     {it : IterM (α := α) m β} {f : β → n (ULift Bool)} {p : β → n (ULift Bool)} :
     (it.filterM f).anyM p = (it.mapM (pure (f := n))).anyM (fun x => do
         if (← f x).down then
@@ -960,7 +1074,16 @@ theorem IterM.anyM_filterM {α β : Type w} {m : Type w → Type w'} {n : Type w
   rw [anyM_eq_match_step, anyM_eq_match_step, step_mapM, step_filterM, bind_assoc, bind_assoc]
   apply bind_congr; intro step
   split
-  · simp only [bind_assoc, pure_bind, Shrink.inflate_deflate]
+  · rename_i out _ _
+    simp only [bind_assoc, pure_bind, Shrink.inflate_deflate]
+    have {x : n (ULift Bool)} : x = MonadAttach.attach (pure out) >>= (fun _ => x) := by
+      rw (occs := [1]) [show x = pure out >>= (fun _ => x) by simp]
+      conv => lhs; rw [← LawfulMonadAttach.map_attach (x := pure out)]
+      simp
+    refine Eq.trans this ?_
+    simp only [LawfulMonadAttach.bind_attach_of_nonempty (x := pure out), pure_bind]
+    split; rotate_left; rfl
+    conv => rhs; rw [← LawfulMonadAttach.map_attach (x := f _), bind_map_left]
     apply bind_congr; intro fx
     split <;> simp [ihy ‹_›]
   · simp only [PlausibleIterStep.skip, pure_bind, bind_assoc]
@@ -1023,8 +1146,9 @@ theorem IterM.anyM_filter {α β : Type w} {m : Type w → Type w'}
   · simp
 
 theorem IterM.any_filterMapM {α β β' : Type w} {m : Type w → Type w'} {n : Type w → Type w''}
-    [Iterator α m β] [Finite α m] [Monad m] [Monad n] [MonadLiftT m n] [IteratorLoop α m m]
-    [LawfulMonad m] [LawfulMonad n] [LawfulMonadLiftT m n] [LawfulIteratorLoop α m m]
+    [Iterator α m β] [Finite α m] [MonadLiftT m n] [IteratorLoop α m m]
+    [Monad m] [LawfulMonad m] [Monad n] [MonadAttach n] [LawfulMonad n] [LawfulMonadAttach n]
+    [LawfulMonadLiftT m n] [LawfulIteratorLoop α m m]
     {it : IterM (α := α) m β} {f : β → n (Option β')} {p : β' → Bool} :
     (it.filterMapM f).any p = (it.mapM (pure (f := n))).anyM (fun x => do
       match ← f x with
@@ -1033,15 +1157,17 @@ theorem IterM.any_filterMapM {α β β' : Type w} {m : Type w → Type w'} {n : 
   simp [any_eq_anyM, anyM_filterMapM]
 
 theorem IterM.any_mapM {α β β' : Type w} {m : Type w → Type w'} {n : Type w → Type w''}
-    [Iterator α m β] [Finite α m] [Monad m] [Monad n] [MonadLiftT m n] [IteratorLoop α m m]
-    [LawfulMonad m] [LawfulMonad n] [LawfulMonadLiftT m n] [LawfulIteratorLoop α m m]
+    [Iterator α m β] [Finite α m] [MonadLiftT m n] [IteratorLoop α m m]
+    [Monad m] [LawfulMonad m] [Monad n] [MonadAttach n] [LawfulMonad n] [LawfulMonadAttach n]
+    [LawfulMonadLiftT m n] [LawfulIteratorLoop α m m]
     {it : IterM (α := α) m β} {f : β → n β'} {p : β' → Bool} :
     (it.mapM f).any p = (it.mapM (pure (f := n))).anyM (fun x => (.up <| p ·) <$> (f x)) := by
   simp [any_eq_anyM, anyM_mapM]
 
 theorem IterM.any_filterM {α β : Type w} {m : Type w → Type w'} {n : Type w → Type w''}
-    [Iterator α m β] [Finite α m] [Monad m] [Monad n] [MonadLiftT m n] [IteratorLoop α m m]
-    [LawfulMonad m] [LawfulMonad n] [LawfulMonadLiftT m n] [LawfulIteratorLoop α m m]
+    [Iterator α m β] [Finite α m] [MonadLiftT m n] [IteratorLoop α m m]
+    [Monad m] [LawfulMonad m] [Monad n] [MonadAttach n] [LawfulMonad n] [LawfulMonadAttach n]
+    [LawfulMonadLiftT m n] [LawfulIteratorLoop α m m]
     {it : IterM (α := α) m β} {f : β → n (ULift Bool)} {p : β → Bool} :
     (it.filterM f).any p = (it.mapM (pure (f := n))).anyM (fun x => do
         if (← f x).down then
@@ -1085,63 +1211,41 @@ theorem IterM.any_map {α β β' : Type w} {m : Type w → Type w'}
   · simp
 
 theorem IterM.allM_filterMapM {α β β' : Type w} {m : Type w → Type w'} {n : Type w → Type w''}
-    [Iterator α m β] [Finite α m] [Monad m] [Monad n] [MonadLiftT m n]
-    [LawfulMonad m] [LawfulMonad n] [LawfulMonadLiftT m n]
+    [Iterator α m β] [Finite α m] [MonadLiftT m n]
+    [Monad m] [LawfulMonad m] [Monad n] [MonadAttach n] [LawfulMonad n] [LawfulMonadAttach n]
+    [LawfulMonadLiftT m n]
     {it : IterM (α := α) m β} {f : β → n (Option β')} {p : β' → n (ULift Bool)} :
     (it.filterMapM f).allM p = (it.mapM (pure (f := n))).allM (fun x => do
       match ← f x with
       | some fx => p fx
       | none => return .up true) := by
-  induction it using IterM.inductSteps with | step it ihy ihs
-  rw [allM_eq_match_step, allM_eq_match_step, step_filterMapM, step_mapM, bind_assoc, bind_assoc]
-  apply bind_congr; intro step
-  split
-  · simp only [bind_assoc, pure_bind, Shrink.inflate_deflate]
-    apply bind_congr; intro fx
-    split
-    · simp [ihy ‹_›]
-    · simp only [PlausibleIterStep.yield, pure_bind, Shrink.inflate_deflate]
-      apply bind_congr; intro px
-      split <;> simp [ihy ‹_›]
-  · simp only [PlausibleIterStep.skip, pure_bind, bind_assoc]
-    simp [ihs ‹_›]
-  · simp
+  rw [allM_eq_not_anyM_not, anyM_filterMapM, allM_eq_not_anyM_not]
+  congr 2; ext x
+  simp only [map_eq_pure_bind, bind_assoc]
+  apply bind_congr; intro y
+  split <;> simp
 
 theorem IterM.allM_mapM {α β β' : Type w} {m : Type w → Type w'} {n : Type w → Type w''}
-    [Iterator α m β] [Finite α m] [Monad m] [Monad n] [MonadLiftT m n]
-    [LawfulMonad m] [LawfulMonad n] [LawfulMonadLiftT m n]
-    {it : IterM (α := α) m β} {f : β → n β'} {p : β' → n (ULift Bool)} :
+    [Iterator α m β] [Finite α m] [MonadLiftT m n]
+    [Monad m] [LawfulMonad m] [Monad n] [MonadAttach n] [LawfulMonad n] [LawfulMonadAttach n]
+    [LawfulMonadLiftT m n] {it : IterM (α := α) m β} {f : β → n β'} {p : β' → n (ULift Bool)} :
     (it.mapM f).allM p = (it.mapM (pure (f := n))).allM (fun x => do p (← f x)) := by
-  induction it using IterM.inductSteps with | step it ihy ihs
-  rw [allM_eq_match_step, allM_eq_match_step, step_mapM, step_mapM, bind_assoc, bind_assoc]
-  apply bind_congr; intro step
-  split
-  · simp only [bind_assoc, pure_bind, Shrink.inflate_deflate]
-    apply bind_congr; intro fx
-    simp [ihy ‹_›]
-  · simp only [PlausibleIterStep.skip, pure_bind, bind_assoc]
-    simp [ihs ‹_›]
-  · simp
+  simp [allM_eq_not_anyM_not, anyM_mapM]
 
 theorem IterM.allM_filterM {α β : Type w} {m : Type w → Type w'} {n : Type w → Type w''}
-    [Iterator α m β] [Finite α m] [Monad m] [Monad n] [MonadLiftT m n]
-    [LawfulMonad m] [LawfulMonad n] [LawfulMonadLiftT m n]
+    [Iterator α m β] [Finite α m] [MonadLiftT m n]
+    [Monad m] [LawfulMonad m] [Monad n] [MonadAttach n] [LawfulMonad n] [LawfulMonadAttach n]
+    [LawfulMonadLiftT m n]
     {it : IterM (α := α) m β} {f : β → n (ULift Bool)} {p : β → n (ULift Bool)} :
     (it.filterM f).allM p = (it.mapM (pure (f := n))).allM (fun x => do
         if (← f x).down then
           p x
         else
           return .up true) := by
-  induction it using IterM.inductSteps with | step it ihy ihs
-  rw [allM_eq_match_step, allM_eq_match_step, step_mapM, step_filterM, bind_assoc, bind_assoc]
-  apply bind_congr; intro step
-  split
-  · simp only [bind_assoc, pure_bind, Shrink.inflate_deflate]
-    apply bind_congr; intro fx
-    split <;> simp [ihy ‹_›]
-  · simp only [PlausibleIterStep.skip, pure_bind, bind_assoc]
-    simp [ihs ‹_›]
-  · simp
+  simp only [allM_eq_not_anyM_not, anyM_filterM, map_bind]
+  congr; ext a
+  apply bind_congr; intro b
+  split <;> simp
 
 theorem IterM.allM_filterMap {α β β' : Type w} {m : Type w → Type w'}
     [Iterator α m β] [Finite α m] [Monad m] [IteratorLoop α m m]
@@ -1151,33 +1255,16 @@ theorem IterM.allM_filterMap {α β β' : Type w} {m : Type w → Type w'}
       match f x with
       | some fx => p fx
       | none => return .up true) := by
-  induction it using IterM.inductSteps with | step it ihy ihs
-  rw [allM_eq_match_step, allM_eq_match_step, step_filterMap, bind_assoc]
-  apply bind_congr; intro step
-  cases step.inflate using PlausibleIterStep.casesOn
-  · simp only
-    split
-    · simp [*, ihy ‹_›]
-    · simp only [*, PlausibleIterStep.yield, pure_bind, Shrink.inflate_deflate]
-      apply bind_congr; intro px
-      split <;> simp [ihy ‹_›]
-  · simp [PlausibleIterStep.skip, pure_bind, ihs ‹_›]
-  · simp
+  simp only [allM_eq_not_anyM_not, anyM_filterMap]
+  congr; ext a
+  split <;> simp
 
 theorem IterM.allM_map {α β β' : Type w} {m : Type w → Type w'}
     [Iterator α m β] [Finite α m] [Monad m] [IteratorLoop α m m]
     [LawfulMonad m] [LawfulIteratorLoop α m m]
     {it : IterM (α := α) m β} {f : β → β'} {p : β' → m (ULift Bool)} :
     (it.map f).allM p = it.allM (fun x => p (f x)) := by
-  induction it using IterM.inductSteps with | step it ihy ihs
-  rw [allM_eq_match_step, allM_eq_match_step, step_map, bind_assoc]
-  apply bind_congr; intro step
-  cases step.inflate using PlausibleIterStep.casesOn
-  · simp only [pure_bind, Shrink.inflate_deflate]
-    apply bind_congr; intro fx
-    simp [ihy ‹_›]
-  · simp [PlausibleIterStep.skip, pure_bind, ihs ‹_›]
-  · simp
+  simp [allM_eq_not_anyM_not, anyM_map]
 
 theorem IterM.allM_filter {α β : Type w} {m : Type w → Type w'}
     [Iterator α m β] [Finite α m] [Monad m][IteratorLoop α m m]
@@ -1188,19 +1275,14 @@ theorem IterM.allM_filter {α β : Type w} {m : Type w → Type w'}
           p x
         else
           return .up true) := by
-  induction it using IterM.inductSteps with | step it ihy ihs
-  rw [allM_eq_match_step, allM_eq_match_step, step_filter, bind_assoc]
-  apply bind_congr; intro step
-  cases step.inflate using PlausibleIterStep.casesOn
-  · simp only
-    split <;> simp [ihy ‹_›]
-  · simp only [PlausibleIterStep.skip, pure_bind]
-    simp [ihs ‹_›]
-  · simp
+  simp only [allM_eq_not_anyM_not, anyM_filter]
+  congr; ext a
+  split <;> simp
 
 theorem IterM.all_filterMapM {α β β' : Type w} {m : Type w → Type w'} {n : Type w → Type w''}
-    [Iterator α m β] [Finite α m] [Monad m] [Monad n] [MonadLiftT m n] [IteratorLoop α m m]
-    [LawfulMonad m] [LawfulMonad n] [LawfulMonadLiftT m n] [LawfulIteratorLoop α m m]
+    [Iterator α m β] [Finite α m] [MonadLiftT m n] [IteratorLoop α m m]
+    [Monad m] [LawfulMonad m] [Monad n] [MonadAttach n] [LawfulMonad n] [LawfulMonadAttach n]
+    [LawfulMonadLiftT m n] [LawfulIteratorLoop α m m]
     {it : IterM (α := α) m β} {f : β → n (Option β')} {p : β' → Bool} :
     (it.filterMapM f).all p = (it.mapM (pure (f := n))).allM (fun x => do
       match ← f x with
@@ -1209,15 +1291,17 @@ theorem IterM.all_filterMapM {α β β' : Type w} {m : Type w → Type w'} {n : 
   simp [all_eq_allM, allM_filterMapM]
 
 theorem IterM.all_mapM {α β β' : Type w} {m : Type w → Type w'} {n : Type w → Type w''}
-    [Iterator α m β] [Finite α m] [Monad m] [Monad n] [MonadLiftT m n] [IteratorLoop α m m]
-    [LawfulMonad m] [LawfulMonad n] [LawfulMonadLiftT m n] [LawfulIteratorLoop α m m]
+    [Iterator α m β] [Finite α m] [MonadLiftT m n] [IteratorLoop α m m]
+    [Monad m] [LawfulMonad m] [Monad n] [MonadAttach n] [LawfulMonad n] [LawfulMonadAttach n]
+    [LawfulMonadLiftT m n] [LawfulIteratorLoop α m m]
     {it : IterM (α := α) m β} {f : β → n β'} {p : β' → Bool} :
     (it.mapM f).all p = (it.mapM (pure (f := n))).allM (fun x => (.up <| p ·) <$> (f x)) := by
   simp [all_eq_allM, allM_mapM]
 
 theorem IterM.all_filterM {α β : Type w} {m : Type w → Type w'} {n : Type w → Type w''}
-    [Iterator α m β] [Finite α m] [Monad m] [Monad n] [MonadLiftT m n] [IteratorLoop α m m]
-    [LawfulMonad m] [LawfulMonad n] [LawfulMonadLiftT m n] [LawfulIteratorLoop α m m]
+    [Iterator α m β] [Finite α m] [MonadLiftT m n] [IteratorLoop α m m]
+    [Monad m] [LawfulMonad m] [Monad n] [MonadAttach n] [LawfulMonad n] [LawfulMonadAttach n]
+    [LawfulMonadLiftT m n] [LawfulIteratorLoop α m m]
     {it : IterM (α := α) m β} {f : β → n (ULift Bool)} {p : β → Bool} :
     (it.filterM f).all p = (it.mapM (pure (f := n))).allM (fun x => do
         if (← f x).down then
@@ -1234,31 +1318,16 @@ theorem IterM.all_filterMap {α β β' : Type w} {m : Type w → Type w'}
       match f x with
       | some fx => (p fx)
       | none => true) := by
-  induction it using IterM.inductSteps with | step it ihy ihs
-  rw [all_eq_match_step, all_eq_match_step, step_filterMap, bind_assoc]
-  apply bind_congr; intro step
-  cases step.inflate using PlausibleIterStep.casesOn
-  · simp only
-    split
-    · simp [*, ihy ‹_›]
-    · simp only [*, PlausibleIterStep.yield, pure_bind, Shrink.inflate_deflate]
-      split <;> simp [ihy ‹_›]
-  · simp [PlausibleIterStep.skip, pure_bind, ihs ‹_›]
-  · simp
+  simp only [all_eq_not_any_not, any_filterMap]
+  congr; ext
+  split <;> simp
 
 theorem IterM.all_map {α β β' : Type w} {m : Type w → Type w'}
     [Iterator α m β] [Finite α m] [Monad m] [IteratorLoop α m m]
     [LawfulMonad m] [LawfulIteratorLoop α m m]
     {it : IterM (α := α) m β} {f : β → β'} {p : β' → Bool} :
     (it.map f).all p = it.all (fun x => p (f x)) := by
-  induction it using IterM.inductSteps with | step it ihy ihs
-  rw [all_eq_match_step, all_eq_match_step, step_map, bind_assoc]
-  apply bind_congr; intro step
-  cases step.inflate using PlausibleIterStep.casesOn
-  · simp only [pure_bind]
-    simp [ihy ‹_›]
-  · simp [PlausibleIterStep.skip, pure_bind, ihs ‹_›]
-  · simp
+  simp [all_eq_not_any_not, any_map]
 
 end AnyAll
 
